Instances.lean
@@ -36,6 +36,8 @@ import Instances.Examples.VexMovEcxEdiFixture
 import Instances.Examples.VexMovEaxEdiFixture
 import Instances.Examples.VexMovRaxMemRdiExample
 import Instances.Examples.VexMovRaxMemRdiFixture
+import Instances.Examples.VexMovzxRaxMemRdiExample
+import Instances.Examples.VexMovzxRaxMemRdiFixture
 import Instances.Examples.VexMovMemRdiRaxExample
 import Instances.Examples.VexMovMemRdiRaxFixture
 import Instances.Examples.VexStore64Example
