Instances/Examples/VexMovEaxEdiFixture.lean
@@ -12,25 +12,33 @@ def bytes : List UInt8 := [0x89, 0xf8]
 def block : Amd64Block :=
   mkAmd64Block [
       .wrTmp 2 (.get .rdi),
-      .wrTmp 1 (.low32 (.tmp 2)),
-      .wrTmp 0 (.uext32 (.tmp 1)),
+      .wrTmp 1 (.narrow32 (.tmp 2)),
+      .wrTmp 0 (.zext64 (.tmp 1)),
       .put .rax (.tmp 0)
     ] 0x400002
 
 def input : Amd64ConcreteState :=
-  mkAmd64State
+  mkAmd64StateCC
     0xdeadbeefdeadbeef
     0x0
     0x1122334455667788
     0x400000
+    0x0
+    0x0
+    0x0
+    0x0
     ByteMem.empty
 
 def expected : Amd64ConcreteState :=
-  mkAmd64State
+  mkAmd64StateCC
     0x55667788
     0x0
     0x1122334455667788
     0x400002
+    0x0
+    0x0
+    0x0
+    0x0
     ByteMem.empty
 
 end Instances.Examples.VexMovEaxEdiFixture
